src/Var.v
@@ -1,0 +1,72 @@
+Require Import Coq.Structures.OrderedType.
+Require Import Coq.Structures.OrderedTypeEx.
+Require Import Coq.FSets.FMapAVL.
+Require Coq.FSets.FMapFacts.
+Require Import Coq.Arith.Peano_dec.
+
+Inductive var := varid : nat -> var.
+
+Definition var_nat r := match r with | varid n => n end.
+
+Module VAR <: UsualOrderedType.
+  Definition t := var.
+  Definition eq := @eq t.
+  Definition lt x y := lt (var_nat x) (var_nat y).
+  Definition eq_refl := @eq_refl t.
+  Definition eq_sym := @eq_sym t.
+  Definition eq_trans := @eq_trans t.
+  Lemma lt_trans: forall x y z : t, lt x y -> lt y z -> lt x z.
+  Proof.
+    intros.
+    unfold lt in *.
+    destruct x, y, z.
+    simpl in *.
+    omega.
+  Qed.
+
+  Lemma lt_not_eq : forall x y : t, lt x y -> ~ eq x y.
+  Proof.
+    unfold lt in *.
+    intros.
+    destruct x, y.
+    simpl in *.
+    unfold not; intros.
+    inversion H0.
+    subst.
+    apply Lt.lt_irrefl in H.
+    inversion H.
+  Qed.
+
+  Require Import Coq.Arith.Compare_dec.
+  Lemma compare:
+    forall x y, Compare lt eq x y.
+  Proof.
+    intros.
+    destruct x, y.
+    destruct (Nat_as_OT.compare n n0);
+    eauto using LT, GT.
+    apply EQ.
+    unfold Nat_as_OT.eq in *.
+    subst.
+    intuition.
+  Qed.
+
+  Lemma eq_dec : forall x y : t, {eq x y} + {~ eq x y}.
+  Proof.
+    intros.
+    unfold eq.
+    destruct x, y.
+    destruct (eq_nat_dec n n0).
+    - subst; eauto.
+    - right.
+      unfold not.
+      intros.
+      contradiction n1.
+      inversion H; auto.
+  Qed.
+End VAR.
+
+
+Module MV := FMapAVL.Make VAR.
+Module MV_Facts := FMapFacts.Facts MV.
+
